on the way towards the subterm criterion

DP/Subterm.v
@@ -8,19 +8,20 @@ Subterm Criterion from
   Dependency Pairs Revisited (Nao Hirokawa and Aart Middeldorp).
 *)
 
-(* $Id: Subterm.v,v 1.2 2008-08-07 14:00:17 blanqui Exp $ *)
+(* $Id: Subterm.v,v 1.3 2008-09-24 10:20:55 joerg Exp $ *)
 
 Set Implicit Arguments.
 
 Require Export ATrs.
 Require Export Union.
+Require Export ACompat.
 
 (***********************************************************************)
 (** Projections. *)
 
 Record Projection (Sig : Signature) : Type := mkProjection {
   pi : forall f : Sig, nat;
-  pi_bound : forall f, pi f <= (@arity Sig f)
+  pi_bound : forall f, pi f < (@arity Sig f)
 }.
 
 Section subterm_criterion.
@@ -31,12 +32,29 @@ Notation term := (term Sig).
 Notation rule := (rule Sig).
 Notation rules := (list rule).
 
-Variable R : rules.
+Definition is_Fun (t : term) : Prop :=
+  match t with
+    | Var x => False
+    | Fun f v => True
+  end.
+
+Definition option_isSome (A : Type) (o : option A) : Prop :=
+  match o with
+    | Some a => True
+    | None => False
+  end.
+
+Definition project (p: Projection Sig) (t : term) : is_Fun t -> term :=
+  match t return (is_Fun t -> term) with
+    | Var x => fun isfun : is_Fun (Var x) => False_rec term isfun
+    | Fun f v => fun _ : is_Fun (Fun f v) => Vnth v (pi_bound p f)
+  end.
 
 (***********************************************************************)
 (* Subterm Criterion from Dependency Pairs Revisited *)
 
 Definition subterm_rel (x y : term) : Prop := subterm x y.
+Definition subterm_eq_rel (x y : term) : Prop := subterm_eq x y.
 
 Lemma subterm_rel_wf : WF (transp subterm_rel).
 
@@ -46,11 +64,11 @@ Proof.
   assert (subterm y x); inversion sy as [c [hole subst]]; auto.
 Qed.
 
-Lemma comm_subterm_reduction :
+Lemma comm_subterm_reduction : forall R : rules,
     (transp subterm_rel) @ (red R) << (red R) @ (transp subterm_rel).
 
 Proof.
-  intros x z [y [xSuby yRz]].
+  intros R x z [y [xSuby yRz]].
   inversion xSuby as [C [notHoleC fillCy]].
   inversion yRz as [l [r [Cred [s [rule [yfillCredl zfillCredr]]]]]].
   exists (fill C z). split.
@@ -61,12 +79,12 @@ Proof.
   exists C. split. assumption. refl.
 Qed.
 
-Lemma subterm_and_reduction_sn : 
+Lemma subterm_and_reduction_sn : forall R : rules,
   forall x : term, 
     SN (red R) x -> SN (red R U (transp subterm_rel)) x.
 
 Proof.
-  intros x snx. apply sn_comm_sn; trivial.
+  intros R x snx. apply sn_comm_sn; trivial.
   intros y _. apply subterm_rel_wf. clear. intros x y xy.
   assert ((red R @ transp subterm_rel) x y) as [z [xz zy]].
   apply comm_subterm_reduction. assumption.
@@ -78,5 +96,38 @@ Qed.
 (** Subterm criterion *)
 
 (** should be an easy consequence of subterm_and_reduction_sn *)
+
+Definition rule_is_Fun (r : rule) := is_Fun (lhs r) /\ is_Fun (rhs r).
+
+Record dprule : Set := mkDPRule { r : rule; proof : rule_is_Fun r }.
+
+(* Working on it
+Lemma subterm_criterion :
+  forall p : Projection Sig, forall R : list dprule, forall R' : list dprule, forall E : rules,
+  lforall (fun rule => (transp subterm_eq_rel) 
+                       (project p (lhs (r rule)) (proj1 (proof rule))) 
+                       (project p (rhs (r rule)) (proj2 (proof rule)))) R
+  -> lforall (fun rule => (transp subterm_rel) 
+                       (project p (lhs (r rule)) (proj1 (proof rule))) 
+                       (project p (rhs (r rule)) (proj2 (proof rule)))) R'
+  -> WF (hd_red_mod_min E (map r R)) -> WF (hd_red_mod_min E (map r (R ++ R'))).
+
+Proof.
+  intros p R R' E subeqR subR' wfR.
+  set (er := hd_red_mod_min E (map r R)). set (er' := hd_red_mod_min E (map r R')).
+  Print lex'.
+  apply WF_incl with (S := lex' (er'!) (er!)).
+  trans (er U succ). trans (er U er'). unfold er, er'. apply hd_red_mod_min_union.
+  union. unfold er', succ. incl_red.
+  trans (succ U er). apply union_commut.
+  trans (succ U er!). union. apply tc_incl.
+  apply lex'_intro. apply WF_lex'. WFtac. apply WF_tc. exact H2. apply tc_trans.
+  apply comp_tc_incl. trans (succ_eq! @ succ). comp. unfold er.
+  trans (red_mod E R). apply incl_trans with (hd_red_mod E R).
+  apply hd_red_mod_min_incl. apply hd_red_mod_incl_red_mod. incl_red.
+  apply comp_tc_incl. rptac.
+
+Qed.
+*)
 
 End subterm_criterion.
